{
 "cells": [
  {
   "cell_type": "markdown",
   "metadata": {},
   "source": [
    "# Logic and proofs\n",
    "\n",
    "Based on [Geoff Gordon's Propositional Logic lecture notes](https://qna.cs.cmu.edu/#/pages/view/143) and [Other Logical systems lecture notes](https://qna.cs.cmu.edu/#/pages/view/165), and on [Mary Radcliffe's Logic and Proofs lecture notes](http://www.math.cmu.edu/~mradclif/teaching/127S19/Notes/Logic%20and%20Proof.pdf)\n",
    "\n",
    "Learning Objectives of this lecture:\n",
    "- understand basic elements of propositional logic and first order logic.\n",
    "- know inference rules\n",
    "- know additional rules of classical logic\n",
    "- use these to construct proofs\n",
    "- be able to use the different proofs techniques\n"
   ]
  },
  {
   "cell_type": "markdown",
   "metadata": {},
   "source": [
    "## Inference rules and proofs\n",
    "\n",
    "To work with statements in propositional logic, we use inference rules. The most famous of these is probably modus ponens: from premises $p$ and $p→q$, conclude $q$.\n",
    "\n",
    "For example: \"Socrates is a man; if Socrates is a man then Socrates is mortal; therefore Socrates is mortal\", we can write\n",
    "\n",
    "\\begin{array}{ll}\n",
    "\\text{man(Socrates)} & \\text{[assumption]}\\\\\n",
    "\\text{man(Socrates)→mortal(Socrates)}&  \\text{[assumption]}\\\\\n",
    "\\text{mortal(Socrates) }    &    \\text{[modus ponens; 1, 2]}\n",
    "\\end{array}\n",
    "\n",
    "The format above is often called a \"two-column proof\": we write statements in the left column, and their justifications in the right column.\n",
    "\n",
    "### Lemmas\n",
    "The above proof demonstrates the statement\n",
    "\n",
    "man(Socrates)∧(man(Socrates)→mortal(Socrates))→mortal(Socrates) \n",
    "\n",
    "To see why, collect all of the proof's assumptions together with ∧, take the last line of the proof as the final conclusion, and write \"assumptions → conclusion\".  (We could actually have taken any line of the proof as the conclusion, but conventionally we put the conclusion last.)\n",
    "\n",
    "This process — summarizing a proof or part of a proof by collecting together its assumptions and conclusion — is called \"implication introduction\" or \"proving a lemma\".  \n",
    "\n",
    "To go with implication introduction, modus ponens is sometimes called \"implication elimination.\"\n",
    "\n",
    "### Other inference rules\n",
    "There are lots of useful inference rules besides implication introduction and implication elimination.  For example:\n",
    "\n",
    "- $\\wedge$ introduction: if we separately prove $p$ and $q$, then that constitutes a proof of $p \\wedge q$.\n",
    "- $\\wedge$ elimination: from $p\\wedge q$ we can conclude either of $p$ and $q$ separately.\n",
    "- $\\vee$ introduction: from $p$ we can conclude $p\\vee q$ for any $q$.\n",
    "- $\\vee$ elimination (also called proof by cases): if we know $p\\vee q$ (the cases) and we have both $p\\rightarrow r$  and $q\\rightarrow r$  (the case-specific proofs), then we can conclude $r$.\n",
    "- T introduction: we can conclude T from no assumptions.\n",
    "- F elimination: from F we can conclude an arbitrary formula $p$. \n",
    "- Associativity: both $\\wedge$ and $\\vee$ are associative: it doesn't matter how we parenthesize an expression like $a\\wedge b\\wedge c\\wedge d$. (So in fact we often just leave the parentheses out in such cases. But when having $\\vee$ and $\\wedge$ together, it's a good idea to keep the parentheses.)\n",
    "- Distributivity: $\\wedge$ and $\\vee$ distribute over one another; for example, $a\\wedge(b\\vee c)$  is equivalent to $(a\\vee b)\\wedge(a\\vee c)$.\n",
    "- Commutativity: both $\\wedge$ and $\\vee$ are commutative (symmetric in the order of their arguments), so we can re-order their arguments however we please.  For example, $a\\wedge b\\wedge c$ is equivalent to $c\\wedge b\\wedge a$.\n",
    "\n",
    "#### Exercise:\n",
    "Prove: $(a\\wedge b)\\rightarrow(b\\wedge a)$\n",
    "\n",
    "\n",
    "### Additional rules for classical logic:\n",
    "(in classical logic we force statments to be either true or false. We will focus in this class on classical logic. In constructive logic, it might be the case that we cannot prove either $p$ or $\\neg p$.\n",
    "\n",
    "##### Law of Excluded Middle\n",
    "\n",
    "\n",
    "Let $p$ be a proposition. Regardless of the truth value of $p$, $p\\vee(\\neg p)$ is always true.\n",
    "\n",
    "To prove this theorem, we consider the following truth table:\n",
    "\n",
    "\\begin{array}{c||c|c}\n",
    "p & \\neg p & p\\vee(\\neg p)\\\\\n",
    "\\hline T & F & T\\\\\n",
    "F & T & T\n",
    "\\end{array}\n",
    "\n",
    "\n",
    "Regardless of the truth value of $p$, we have that $p\\vee (\\neg p)$ is always true. This is an example of a tautology. A propositional formula is called a tautology if the formula is true, regardless of the truth values of the propositional variables from which it is constructed. \n",
    "\n",
    "##### De Morgan's Laws\n",
    "Let $p, q$ be propositional variables. Then\n",
    "- $\\neg(p\\wedge q) \\equiv (\\neg p)\\vee(\\neg q)$\n",
    "- $\\neg(p\\vee q)\\equiv (\\neg p)\\wedge (\\neg q)$\n",
    "\n",
    "\n",
    "A full proof of this theorem is left as an exercise.\n",
    "Another exercise: Show that the propositional formula $(\\neg p)\\wedge (\\neg(p\\wedge q))$ is logically equivalent to $\\neg p$.\n",
    "\n",
    "\n",
    "##### Double negation elimination: \n",
    "\n",
    "$\\neg\\neg p$ is equivalent to $p$.\n",
    "\n",
    "##### Contraposition: \n",
    "\n",
    "$p\\rightarrow q$ is equivalent to $\\neg q\\rightarrow \\neg p$.\n",
    "\n",
    "All of these are equivalent: from any one of these (plus the inference rules above) we can prove the others."
   ]
  },
  {
   "cell_type": "markdown",
   "metadata": {},
   "source": [
    "#### Exercise \n",
    "Show using the definition of $p\\rightarrow q$ that $ p\\rightarrow q \\equiv \\neg(p\\wedge(\\neg q)) \\equiv (\\neg p)\\vee q,$\n"
   ]
  },
  {
   "cell_type": "markdown",
   "metadata": {},
   "source": [
    "### Complex proofs and scoping rules\n",
    "\n",
    "Here is a proof that $[PB\\wedge J\\to\\textit{Sandwich}]\\to[PB\\to (J\\to\\textit{Sandwich})]$. The way you read it is: \"Suppose that peanut butter and jelly together make a sandwich.  Then, if you give me peanut butter, it will mean that jelly is enough to make a sandwich.\"\n",
    "\n",
    "We write the proof below while following scoping rules. Assumptions made outside a lemma in an enclosing scope are available inside the scope of that lemma, but are not used in its result. Assumptions made inside the lemma are no longer used outside.\n",
    "\n",
    "Proof:\n",
    "\n",
    "- 1- Lemma:\n",
    "    - 1- Assume: $PB∧J→Sandwich$\n",
    "    - 2- Lemma:  \n",
    "        - 1- Assume: $PB$\n",
    "        - 2- Lemma: \n",
    "            - 1- Assume: $J$\n",
    "            - 2- $PB∧J$  [from 1.2.1, 1.2.2.1, ∧-introduction]\n",
    "            - 3- $\\textit{Sandwich}$ [from 1.2.2.2, 1, modus ponens]\n",
    "        - 3- End lemma: $J\\rightarrow\\textit{Sandwich}$\n",
    "    - 3- End lemma: $PB\\rightarrow(J\\rightarrow\\textit{Sandwich})$\n",
    "- 2- End lemma:$[PB∧J\\rightarrow\\textit{Sandwich}]\\rightarrow[PB\\rightarrow(J\\rightarrow\\textit{Sandwich})]$"
   ]
  },
  {
   "cell_type": "markdown",
   "metadata": {},
   "source": [
    "### Resolution\n",
    "\n",
    "A useful inference rule — one that is not as well known as some — is resolution. \n",
    "\n",
    "Suppose we have two statments such as: $p\\vee r$ and $\\neg p\\vee q$.\n",
    "\n",
    "Resolution lets us conclude $q\\vee r$.\n",
    "\n",
    "We can also apply it for more complex clauses:\n",
    "\n",
    "From $a\\vee b \\vee c \\vee d $ and $b \\vee \\neg c \\vee s \\vee t$ we can conclude: $a\\vee b \\vee s \\vee t $ .\n",
    "\n",
    "The conclusion contains every literal that was in either of the two original clauses, except for d and ¬d. (The literal b appears in both input clauses, but only shows up once in the output, since $b\\vee b \\equiv b$."
   ]
  },
  {
   "cell_type": "markdown",
   "metadata": {},
   "source": [
    "#### Exercise\n",
    "\n",
    "From [notes](https://qna.cs.cmu.edu/#/pages/view/143)\n",
    "\n",
    "\"In mini sudoku, the digits 1..4 must appear exactly once in each row, column, and bold-edged 2*2 box of the grid.  In the grid below, we've been given five fixed digits (e.g., the 3 in the upper right corner).  The squares labeled a, b, c, d are currently blank, and we'd like to figure out how to fill them in:\n",
    "\n",
    "\\begin{array}{cc||cc} \n",
    "1&&&3\\\\\n",
    "&&&2\\\\\n",
    "\\hline\n",
    "&3&a&b\\\\\n",
    "&1&c&d\\\\\n",
    "\\end{array}\n",
    "\n",
    "For example, we know that square d can't contain the digit 2, because there's already a 2 directly above it in the same column.\n",
    "\n",
    "Fill in the squares a, b, c, d.  (Note: no guessing is required.)\n",
    "\n",
    "Use the rules of propositional logic to write down the constraints that squares a, b, c, d must satisfy.  For example, you should write that the digit 1 must appear exactly once in the squares a, b, c, d.  (It may take several logical formulas to implement this constraint.)  For another example, you should write that the digit 2 can't appear in squares b or d (because of the 2 above them in the same column).\n",
    "\n",
    "Prove that the solution you gave above is correct, using your formulation of the constraints together with the rules of propositional logic.\""
   ]
  },
  {
   "cell_type": "markdown",
   "metadata": {
    "collapsed": true
   },
   "source": [
    "# First-order logic\n",
    "\n",
    "First-order logic can group together multiple propositions related to an object. Each proposition is then a Boolean-valued function applied to the object and is called a predicate or a property.\n",
    "\n",
    "For example, the object can be socrates and the Boolean properties can be man, mortal, etc.:\n",
    "\n",
    "- $man(Socrates)=T$\n",
    "- $mortal(Socrates)=T$\n",
    "- $Greek(Socrates)=T$\n",
    "- $Roman(Socrates)=F$\n",
    "\n",
    "\n",
    "We can use logical connective to connect these properties:\n",
    "\n",
    "$$(man(Socrates)∧mortal(Socrates))∨Roman(Socrates)$$\n",
    "\n",
    "And define the same properties for another object like Caesar, but with other true values:\n",
    "\n",
    "- $man(Caesar)=T$\n",
    "- $mortal(Caesar)=T$\n",
    "- $Greek(Caesar)=F$\n",
    "- $Roman(Caesar)= T$\n",
    "\n",
    "\n",
    "We can also have properties associated with tuples of objects, such as:\n",
    "\n",
    "$$friends(Socrates,Plato)=T$$\n",
    "\n",
    "\n",
    "### Functions\n",
    "First-order logic also includes functions that act on objects or tuples of objects. For example:\n",
    "\n",
    "$$ advisor(Plato)=Socrates$$\n",
    "\n",
    "Functions return objects. It makes sense to nest a function in a property (such as $Greek(advisor(Plato)))=T$) but not the other way around\n",
    "\n",
    "### Inference rules\n",
    "\n",
    "Bu adding objects and functions, we can prove things for many propositions at once, such as proving that $man(x)→mortal(x)$ is true for any object x, whereas in propositional logic we could only prove things about specific propositions.\n",
    "\n",
    "### Reasoning and theories.\n",
    "\n",
    "There are many different resoning theories with different facts and different kinds of reasoning. But the basic structure of expressing a proof as a sequence of statements (either assumptions or conclusions from applying a rule) is the same. \n",
    "\n",
    "Each logic has a theory (a list of new objects, predicates, functions, and facts, together with inference rules for reasoning about them).  For example, we might design a theory of real numbers, which would introduce objects like $1.4$, $\\pi$, and $−27$, along with functions like $+$ and $⋅$, and facts like $0\\in\\mathbb{R}$. To work with statements in this theory of reals, we might use inference rules like linear combination of equations. The new facts in a theory are often called axioms; we can think of them as inference rules with no premises.\n"
   ]
  },
  {
   "cell_type": "markdown",
   "metadata": {},
   "source": [
    "# Proof Techniques: \n",
    "\n",
    "### Direct proof\n",
    "\n",
    "Direct Proof of $p\\rightarrow q$\n",
    "- Assume $p$ to be true.\n",
    "-  Conclude that $r_1$ must be true (for some $r_1$).\n",
    "- Conclude that $r_2$ must be true (for some $r_2$).\n",
    "- $\\vdots$\n",
    "- Conclude that $r_k$ must be true (for some $r_k$).\n",
    "- Conclude that $q$ must be true.\n",
    "\n",
    "\n",
    "Prove that: If $a$ and $b$ are consecutive integers, then $a + b$ is odd.\n",
    "\n",
    "### Proof by Cases\n",
    "(if we know $p\\vee q$ (the cases) and we have both $p\\rightarrow r$  and $q\\rightarrow r$  (the case-specific proofs), then we can conclude $r$)\n",
    "\n",
    "Proof of $p\\rightarrow q$ by Cases.\n",
    "- Write $p \\equiv r_1 \\vee r_2\\vee \\dots\\vee r_k$.\n",
    "- Separately prove $r_i\\rightarrow q$ for each $i$, using any method.\n",
    "- Conclude that $p\\rightarrow q$, since $p\\rightarrow q \\equiv (r_1\\rightarrow q)\\wedge (r_2\\rightarrow q)\\wedge \\dots (r_k\\rightarrow q)$.\n",
    "\n",
    "Prove that: If $x$ is a real number, then $|x + 3| − x > 2$.\n",
    "\n",
    "### Proof by Contradiction\n",
    "\n",
    "Proof of $p$ by Contradiction\n",
    "- Assume $p$ is false.\n",
    "- Follow the method of Direct Proof to conclude that $q$ must be true (for some $q$ that is observably false).\n",
    "- Conclude that $p$ cannot be false.\n",
    "- Conclude that $p$ is therefore true.\n",
    "\n",
    "\n",
    "Prove that: There is no smallest positive rational number.\n",
    "\n",
    "\n",
    "### Proof by Contraposition\n",
    "\n",
    "\\begin{eqnarray*}\n",
    "p\\rightarrow q & \\equiv & \\neg(p\\wedge (\\neg q))\\\\\n",
    " & \\equiv & \\neg( (\\neg q)\\wedge p)\\\\\n",
    " & \\equiv & \\neg ((\\neg q)\\wedge \\neg(\\neg p))\\\\\n",
    " & \\equiv & (\\neg q) \\rightarrow (\\neg p)\n",
    "\\end{eqnarray*}\n",
    "\n",
    "\n",
    "Proof of $p\\rightarrow q$ by Contrapositive:\n",
    "- Assume $q$ is false.\n",
    "- Follow the method of Direct Proof to conclude that $p$ is also false.\n",
    "- Conclude that $\\neg q \\rightarrow \\neg p$ is true.\n",
    "- Since $(\\neg q\\rightarrow \\neg p )\\equiv (p\\rightarrow q)$, conclude that $p\\rightarrow q$ is true.\n",
    "\n",
    "Prove that: Let a, b be integers. If ab is even, then at least one of a or b is even.\n",
    "\n",
    "\n",
    "### Proof by Induction\n",
    "\n",
    "Proof of $P(n)$ is true by Contrapositive:\n",
    "- Show  P(n) is true for some basis case.\n",
    "- Assume that P(n) is true for  n,  show that this implies that P(n + 1) is true.\n",
    "- Then, by the principle of induction, conclude P(n) is true for all n greater or equal to the basis case.\n"
   ]
  },
  {
   "cell_type": "code",
   "execution_count": null,
   "metadata": {
    "collapsed": true
   },
   "outputs": [],
   "source": []
  }
 ],
 "metadata": {
  "kernelspec": {
   "display_name": "Python 3",
   "language": "python",
   "name": "python3"
  },
  "language_info": {
   "codemirror_mode": {
    "name": "ipython",
    "version": 3
   },
   "file_extension": ".py",
   "mimetype": "text/x-python",
   "name": "python",
   "nbconvert_exporter": "python",
   "pygments_lexer": "ipython3",
   "version": "3.5.2"
  }
 },
 "nbformat": 4,
 "nbformat_minor": 2
}
